Op/Inner_M1.v
@@ -5,13 +5,13 @@ Require Import Recdef.
 Local Open Scope Z.
 
 Definition local_update_M (j:nat) (a:Z) (b : list Z) (x:Z) := a * ( from_option id 0 (b !! j)) + x.
-Definition update_M_i_j (i j a:Z) b o := alter (local_update_M (Z.to_nat j) a b) (Z.to_nat (i + j)) o.
+(* Definition update_M_i_j (i j a:Z) b (o:Z) := alter (local_update_M (Z.to_nat j) a b) (Z.to_nat (i + j)) o. *)
 Definition update_M_i_j' (i j:nat) (a:Z) b o := list_alter (local_update_M j a b) (i + j)%nat o.
 
-Function inner_M_fix (i j a:Z) (b o : list Z) {measure Z.to_nat j} : list Z :=
+(* Function inner_M_fix (i j a:Z) (b o : list Z) {measure Z.to_nat j} : list Z :=
   if (j <=? 0) then o else inner_M_fix i (j - 1) a b (update_M_i_j i (j - 1) a b o).
-Proof. intros. apply Z2Nat.inj_lt ; rewrite Z.leb_gt in teq; omega. Defined.
-
+Proof. intros. apply Z2Nat.inj_lt ; move: teq; rewrite Z.leb_gt => teq; omega. Defined.
+ *)
 Fixpoint inner_M_fix' (i j : nat) (a:Z) (b o : list Z) := match j with
   | 0%nat => o
   | S p => inner_M_fix' i p a b (update_M_i_j' i p a b o)
@@ -19,7 +19,7 @@ end.
 
 Function inner_M_fix'' (i j a:Z) (b o : list Z) {measure Z.to_nat j} : list Z :=
   if (j <=? 0) then o else update_M_i_j i (j - 1) a b (inner_M_fix'' i (j - 1) a b o).
-Proof. intros. apply Z2Nat.inj_lt ; rewrite Z.leb_gt in teq; omega. Qed.
+Proof. intros. apply Z2Nat.inj_lt ; move: teq; rewrite Z.leb_gt => teq; omega. Qed.
 
 Lemma update_M_i_j_eq : forall (i j a:Z) (b o: list Z),
   0 <= i ->
@@ -91,18 +91,17 @@ Proof.
   gen b o.
   apply (natlike_ind (fun j => ∀ b o : list ℤ, inner_M_fix i j a b o = inner_M_fix'' i j a b o)) ; try omega.
   - intros ; rewrite inner_M_fix_equation ; rewrite inner_M_fix''_equation ; auto.
-  - clear Hj j ; intros j Hj iHj b o ; sort.
+  - clear Hj j => j Hj iHj b o ; sort.
     change (Z.succ j) with (j + 1).
     rewrite inner_M_fix_equation ; rewrite inner_M_fix''_equation.
     flatten.
-    replace (j + 1 - 1) with (j) by omega.
+    rep_omega (j + 1 - 1) (j).
     rewrite iHj.
     rewrite inner_M_fix''_equation ; symmetry ; rewrite inner_M_fix''_equation.
     flatten.
     apply Z.leb_gt in Eq0.
     rewrite <- inner_M_fix''_com by omega.
-    rewrite update_M_i_j_comm_j by omega.
-    reflexivity.
+    rewrite update_M_i_j_comm_j ; try reflexivity ; omega.
 Qed.
 
 Lemma inner_M_fix_0 : forall i a b o, 0 <= i -> inner_M_fix i 0 a b o = o.
@@ -111,12 +110,12 @@ Proof. intros ; rewrite inner_M_fix_equation ; flatten ; compute in Eq ; tryfals
 Lemma inner_M_fix_step j : 0 <= j -> forall i a b o, 0 <= i -> inner_M_fix i (j + 1) a b o = update_M_i_j i j a b (inner_M_fix i j a b o).
 Proof.
   intros.
-  rewrite inner_M_i_j_eq'' by omega.
+  rewrite inner_M_i_j_eq'' ; try omega.
   rewrite inner_M_fix''_equation.
   flatten.
   apply Zle_bool_imp_le in Eq ; omega. (* silly case *)
   apply Z.leb_gt in Eq.
-  replace (j + 1 - 1) with (j) by omega.
+  rep_omega (j + 1 - 1)  (j).
   rewrite inner_M_i_j_eq''; go.
 Qed.
 
@@ -144,30 +143,29 @@ Proof.
 intros i j a b o Hj Hi. gen i a b o.
 eapply (natlike_ind (fun j => ∀ i : ℤ, 0 ≤ i → ∀ (a : ℤ) (b o : list ℤ),
   i ≤ length o → inner_M_fix i j a b o = take (Z.to_nat i) o ++ drop (Z.to_nat i) (inner_M_fix i j a b o))) ; try omega.
-intros; rewrite inner_M_fix_0 by omega; rewrite take_drop; reflexivity.
-clear j Hj. intros j Hj iHj i Hi a b o Ho.
+intros; rewrite inner_M_fix_0 ; try omega; rewrite take_drop; reflexivity.
+clear j Hj => j Hj iHj i Hi a b o Ho.
 change (Z.succ j) with (j + 1).
-rewrite inner_M_i_j_eq'' by omega.
+rewrite inner_M_i_j_eq''; try omega.
 rewrite inner_M_fix''_equation.
 flatten.
 rewrite take_drop; reflexivity.
-replace (j + 1 - 1) with j by omega.
-rewrite <- inner_M_i_j_eq'' by omega.
-rewrite iHj by omega.
+rep_omega (j + 1 - 1) j.
+rewrite <- inner_M_i_j_eq'' ; try omega.
+rewrite iHj ; try omega.
 unfold update_M_i_j.
 rewrite alter_app_r_alt.
 f_equal.
 
 Focus 2.
-rewrite take_length ; rewrite Z2Nat.inj_add by omega.
+rewrite take_length ; rewrite Z2Nat.inj_add ; try omega.
 apply (NPeano.Nat.le_trans _ (Z.to_nat i)) ; try omega.
 apply Min.le_min_l.
 
-rewrite drop_app_ge by (rewrite take_length ; apply Min.le_min_l).
+rewrite drop_app_ge. 2: (rewrite take_length ; apply Min.le_min_l).
 replace ((Z.to_nat i - length (take (Z.to_nat i) o)))%nat with 0%nat.
 reflexivity.
-rewrite take_length.
-rewrite min_l ; go.
+rewrite take_length min_l ; go.
 rewrite <- Nat2Z.id ; apply Z2Nat.inj_le ; go.
 Qed.
 
@@ -180,28 +178,25 @@ replace i with 0 ; replace j with 0 ; subst ; repeat rewrite inner_M_fix_0 ; go.
   apply (natlike_ind (fun j => ∀ i : ℤ, 0 ≤ i → ∀ (a : ℤ) (b o' : list ℤ),
   i + j <= length (o ++ [h]) → inner_M_fix i j a b ((o ++ [h]) ++ o') = inner_M_fix i j a b (o ++ [h]) ++ o')) ; try omega.
   intros.
-  repeat rewrite inner_M_fix_0 by omega ; reflexivity.
+  repeat (rewrite inner_M_fix_0 ; try omega) ; reflexivity.
   clear j Hj; intros j Hj iHj i Hi a b o' Hijo.
   change (Z.succ j) with (j + 1).
-  repeat rewrite inner_M_i_j_eq'' by omega.
+  repeat (rewrite inner_M_i_j_eq'' ; try omega).
   rewrite inner_M_fix''_equation ; symmetry ; rewrite inner_M_fix''_equation.
   flatten.
   replace (j + 1 - 1) with j by omega.
-  repeat rewrite <- inner_M_i_j_eq'' by omega.
+  repeat (rewrite <- inner_M_i_j_eq'' ; try omega).
   change (Z.succ j) with (j + 1) in *.
   assert(Hijo': i + j <= length o) by (rewrite app_length in Hijo ; simpl in Hijo ; lia).
   clear Hijo.
   unfold update_M_i_j.
   rewrite <- alter_app_l.
   f_equal.
-  rewrite <- app_assoc.
-  rewrite <- cons_middle.
-  rewrite iHo by omega.
-  rewrite iHo by omega.
-  rewrite app_assoc_reverse.
-  rewrite cons_middle.
+  rewrite -app_assoc -cons_middle iHo ; try omega.
+  rewrite iHo ; try omega.
+  rewrite app_assoc_reverse cons_middle.
   reflexivity.
-  rewrite inner_M_fix_length by omega.
+  rewrite inner_M_fix_length ; try omega.
   rewrite app_length.
   rewrite <- Nat2Z.id.
   simpl.
@@ -215,12 +210,11 @@ Proof.
   rewrite <- (take_drop (Z.to_nat (i + j)) o).
   rewrite inner_M_fix_app ; try omega.
   rewrite (take_drop (Z.to_nat (i + j)) o).
-  2: rewrite take_length ; rewrite Nat2Z.inj_min ; rewrite Z.min_l ; rewrite Z2Nat.id ; omega.
+  2: rewrite take_length Nat2Z.inj_min Z.min_l Z2Nat.id ; omega.
   rewrite take_app_ge.
-  2: rewrite inner_M_fix_length by omega ; rewrite take_length ; apply Min.le_min_l.
-  rewrite inner_M_fix_length by omega.
-  rewrite take_length.
-  rewrite min_l.
+  2: rewrite inner_M_fix_length ; try omega ; rewrite take_length ; apply Min.le_min_l.
+  rewrite inner_M_fix_length ; try omega.
+  rewrite take_length min_l.
   2: rewrite <- Nat2Z.id; apply Z2Nat.inj_le; omega.
   replace ((Z.to_nat (i + j) - Z.to_nat (i + j))%nat) with 0%nat by omega.
   replace (take 0 (drop (Z.to_nat (i + j)) o)) with (nil:list Z) by reflexivity.
@@ -236,17 +230,17 @@ Proof.
   - rewrite inner_M_fix_app ; try omega.
     2: rewrite take_length; rewrite min_l.
     2: rewrite Z2Nat.id ; omega.
-    2: rewrite Z2Nat.inj_le in H by omega ; rewrite (Nat2Z.id (length o)) in H ; omega.
-    rewrite inner_M_fix_take by omega ; reflexivity.
+    2: move : H ; rewrite Z2Nat.inj_le ; try omega ; rewrite (Nat2Z.id (length o)) => H ; omega.
+    rewrite inner_M_fix_take ; try omega ; reflexivity.
   - 
   repeat match goal with
     | _ => reflexivity
     | _ => rewrite drop_ge
     | _ => rewrite take_ge
     | _ => rewrite app_nil_r
-    | _ => rewrite inner_M_fix_length by omega
-  end ; 
-  apply Z.gt_lt_iff in H ; rewrite Z2Nat.inj_lt in H by omega ; rewrite (Nat2Z.id (length o)) in H ; omega.
+    | _ => rewrite inner_M_fix_length ; try omega
+  end ;
+  apply Z.gt_lt_iff in H ; move: H ; rewrite Z2Nat.inj_lt ; try omega ; rewrite (Nat2Z.id (length o)) => H ; omega.
 Qed.
 
 Lemma inner_M_fix'_app_drop : forall i j a b o, inner_M_fix' i j a b o = take (i + j)%nat (inner_M_fix' i j a b o) ++ drop (i + j)%nat o.
@@ -289,7 +283,7 @@ m1 ≤ a ∧ a ≤ n1 → m1 ≤ 0 ∧ 0 ≤ n1 → m2 ≤ 0 ∧ 0 ≤ n2 → Fo
                 → Forall (λ x : ℤ, p ≤ x ∧ x ≤ q) (inner_M_fix i j a b o)
 )) ; try omega.
    - intros a b o p q Ha Hm1n1 Hm2n2 Hb Ho Hlb Hlo Hp Hq.
-    rewrite inner_M_fix_0 by omega.
+    rewrite inner_M_fix_0 ; try omega.
     assert(Hpmin:= min_prod_neg_le m1 n1 m2 n2 Hm1n1 Hm2n2).
     assert(Hqmax:= max_prod_pos_le m1 n1 m2 n2 Hm1n1 Hm2n2).
     eapply Forall_impl.
@@ -302,29 +296,25 @@ m1 ≤ a ∧ a ≤ n1 → m1 ≤ 0 ∧ 0 ≤ n1 → m2 ≤ 0 ∧ 0 ≤ n2 → Fo
     assert(Hpmin:= min_prod_neg_le m1 n1 m2 n2 Hm1n1 Hm2n2).
     assert(Hqmax:= max_prod_pos_le m1 n1 m2 n2 Hm1n1 Hm2n2).
     change (Z.succ j) with (j + 1).
-    rewrite inner_M_fix_step by omega.
-    rewrite inner_M_fix_app_drop by omega.
+    rewrite inner_M_fix_step ; try omega.
+    rewrite inner_M_fix_app_drop ; try omega.
     unfold update_M_i_j.
     rewrite alter_app_r_alt.
     + apply Forall_app_2.
       apply Forall_take ; apply iHj ; go.
       assert((Z.to_nat (i + j) <= 31)%nat \/ (31 < Z.to_nat (i + j))%nat) by omega.
       destruct H.
-      * rewrite take_length.
-        rewrite inner_M_fix_length by omega.
-        rewrite min_l by omega.
+      * rewrite take_length inner_M_fix_length ; try omega.
+        rewrite min_l ; try omega.
         replace ((Z.to_nat (i + j) - Z.to_nat (i + j))%nat) with 0%nat by omega.
         apply le_lt_eq_dec in H.
         destruct H.
         (* get rid of second case: list is empty *)
-        2: rewrite e ; rewrite drop_ge ; go.
+        2: rewrite e  drop_ge ; go.
         remember (drop (Z.to_nat (i + j)) o) as t.
         destruct t.
         apply (f_equal (λ x, length x)) in Heqt.
-        rewrite drop_length in Heqt.
-        rewrite Hlo in Heqt.
-        simpl in Heqt.
-        omega.
+        move: Heqt ; rewrite drop_length Hlo //=.
         (* first case where the list is empty is not possible *)
         assert(Hzw: Forall (λ x : ℤ, m3 ≤ x ∧ x ≤ n3) (z::t)).
           rewrite Heqt.
