Libs/List_Decidable.v
@@ -1,0 +1,406 @@
+Set Warnings "-notation-overridden".
+
+Require Export Coq.ZArith.ZArith.
+Require Export Coq.Lists.List.
+Require Import Coq.Sorting.Sorting Orders.
+Require Import ssreflect.
+
+Record environment := { vars : positive -> Z }.
+
+Open Scope Z_scope.
+
+Inductive term :=
+  | Var   : positive -> term
+  | Val   : Z -> term
+  .
+
+Inductive expr :=
+  | R : term -> expr
+  | A : expr -> expr -> expr
+  | M : term -> term -> expr.
+
+Inductive formula := 
+  | Eq : expr -> expr -> formula
+  | LEq : list expr -> list expr -> formula.
+
+Definition term_eqb (x y : term) : bool := match x , y with
+  | Var x , Var y => Pos.eqb x y
+  | Val x,  Val y => Z.eqb x y
+  | _ , _ => false
+  end.
+
+Lemma term_eqb_com : forall x y, term_eqb x y = term_eqb y x.
+Proof.
+move => [] a [] b //=.
+rewrite ?Pos2Z.inj_eqb.
+apply Z.eqb_sym.
+apply Z.eqb_sym.
+Qed.
+
+Lemma term_eqb_refl : forall x y, term_eqb x y = true <-> x = y.
+Proof.
+move => x y ; rewrite /term_eqb ; split => H ; simpl.
+destruct x,y; move: H.
+rewrite Pos.eqb_eq => -> //.
+discriminate.
+discriminate.
+rewrite Z.eqb_eq => -> //.
+subst ; destruct y.
+rewrite Pos.eqb_eq //.
+rewrite Z.eqb_eq //.
+Qed.
+
+
+Definition term_leb (x y : term) : bool := match x , y with
+  | Var x , Var y => Pos.leb x y
+  | Val x , Val y => Z.leb x y
+  | Var x,  Val y => false
+  | Val x,  Var y => true
+  end.
+
+Definition term_ltb (x y : term) : bool := match x , y with
+  | Var x , Var y => Pos.ltb x y
+  | Val x , Val y => Z.ltb x y
+  | Var x,  Val y => false
+  | Val x,  Var y => true
+  end.
+
+Definition term_denote env (x : term) : Z :=
+  match x with
+  | Var n => vars env n
+  | Val n => n
+  end.
+
+Fixpoint expr_denote env (m : expr) : Z :=
+  match m with
+  | R v   => term_denote env v
+  | A x y => (expr_denote env x + expr_denote env y)%Z
+  | M x y => (term_denote env x * term_denote env y)%Z
+  end.
+
+Fixpoint list_expr_denote env (l: list expr) : list Z :=
+  match l with
+    | nil => nil
+    | h :: q => (expr_denote env h) :: list_expr_denote env q
+  end.
+
+Definition formula_denote env (t : formula) : Prop :=
+  match t with
+  | Eq x y     => expr_denote env x = expr_denote env y
+  | LEq x y    => list_expr_denote env x = list_expr_denote env y
+  end.
+
+(*
+Fixpoint expr_size (t : expr) : nat :=
+  match t with
+  | R _ => 1%nat
+  | M x y => 1%nat
+  | A x y => 1%nat + expr_size x + expr_size y
+  end.
+
+Lemma all_expr_have_size t : (0 < expr_size t)%nat.
+Proof. induction t; simpl; omega. Qed.
+*)
+
+Fixpoint flatten_expr (e : expr) : (list (list term)) := match e with
+  | A a b => flatten_expr a ++ flatten_expr b
+  | M a b => (a :: b :: nil) :: nil
+  | R x => (x :: nil) :: nil
+end.
+
+Fixpoint ldenote_M env (ls : list term) : Z :=
+  match ls with
+    | nil => 1
+    | x :: ls' => term_denote env x * (ldenote_M env ls')
+  end.
+
+Lemma ldenote_M_cons: forall env a l, ldenote_M env (a::l) = (term_denote env a) * ldenote_M env l.
+Proof. by move=> //. Qed.
+
+Lemma ldenote_M_app: forall env a b, ldenote_M env (a ++ b) = ldenote_M env a * ldenote_M env b.
+Proof. induction a ; intros ; simpl => //.
+destruct (ldenote_M env b) ; auto.
+rewrite IHa ; ring. Qed.
+
+Fixpoint ldenote env (ls : list (list term)) : Z :=
+  match ls with
+    | nil => 0
+    | x :: ls' => (ldenote_M env x) + (ldenote env ls')
+  end.
+
+Lemma ldenote_cons: forall env a l, ldenote env (a::l) = (ldenote_M env a) + ldenote env l.
+Proof. by move=> //. Qed.
+
+Lemma ldenote_app: forall env a b, ldenote env (a ++ b) = ldenote env a + ldenote env b.
+Proof.
+induction a ; intros ; simpl => //.
+rewrite IHa ; ring.
+Qed.
+
+Lemma flatten_expr_correct : forall env t, expr_denote env t = ldenote env (flatten_expr t).
+Proof.
+induction t ; simpl ; try ring.
+rewrite ldenote_app IHt1 IHt2 => //.
+Qed.
+
+
+
+(*****************************************************************************************
+ *   SORT THE LIST
+ *)
+
+Module TermOrder <: TotalLeBool.
+  Definition t := term.
+  Definition leb x y := term_leb x y.
+
+  Theorem leb_total : forall a1 a2, leb a1 a2 = true \/ leb a2 a1 = true.
+  Proof.
+    move=> a b.
+    unfold leb, term_leb.
+    destruct a, b.
+    rewrite !Pos2Z.inj_leb.
+    assert(H:= Zle_bool_total (Z.pos p) (Z.pos p0)).
+    destruct H as [H|H] ; rewrite H ; auto.
+    by right.
+    by left.
+    assert(H:= Zle_bool_total z z0).
+    destruct H as [H|H] ; rewrite H ; auto.
+  Qed.
+
+End TermOrder.
+
+Module ListTermOrder <: TotalLeBool.
+  Definition t := list term.
+
+  Fixpoint leb x y := match x, y with
+    | nil , _ => true
+    | _ , nil => false
+    | a :: qa, b :: qb => match term_ltb a b with
+      | true => true
+      | false => match term_eqb a b with
+        | true => leb qa qb
+        | false => false
+        end
+      end
+  end.
+
+  Theorem leb_total : forall a1 a2, leb a1 a2 = true \/ leb a2 a1 = true.
+  Proof.
+  elim => [| a qa IHa].
+  by left.
+  move=> [| b qb] ; simpl.
+  by right.
+  specialize IHa with qb ; simpl.
+  destruct(term_ltb a b) eqn:H0 ; destruct(term_ltb b a) eqn:H1.
+  by left.
+  by left.
+  by right.
+  destruct(term_eqb a b) eqn:H2; destruct(term_eqb b a) eqn:H3.
+  auto.
+  move: H3 ; rewrite term_eqb_com; congruence.
+  move: H3 ; rewrite term_eqb_com; congruence.
+  exfalso.
+  clear IHa.
+  unfold term_ltb, term_eqb in *.
+  destruct a, b ; try discriminate.
+  move: H2 ; rewrite Pos2Z.inj_eqb Z.eqb_neq.
+  move: H0 ; rewrite Pos2Z.inj_ltb Z.ltb_ge.
+  move: H1 ; rewrite Pos2Z.inj_ltb Z.ltb_ge.
+  move => ? ? ?.
+  omega.
+  move: H2 ; rewrite Z.eqb_neq.
+  move: H0 ; rewrite Z.ltb_ge.
+  move: H1 ; rewrite Z.ltb_ge.
+  move => ? ? ?.
+  omega.
+  Qed.
+End ListTermOrder.
+
+Module Import TermSort := Sort TermOrder.
+
+Lemma perm_ldenote_M : forall env l l', Permutation.Permutation l l' -> ldenote_M env l = ldenote_M env l'.
+Proof.
+  intros env l l' H.
+  induction H => // ; simpl.
+  by rewrite IHPermutation.
+  ring.
+  by rewrite IHPermutation1 IHPermutation2.
+Qed.
+
+Lemma sort_ldenote_M : forall env l, ldenote_M env l = ldenote_M env (TermSort.sort l).
+Proof.
+  intros.
+  apply perm_ldenote_M.
+  apply Permuted_sort.
+Qed.
+
+Module Import ListTermSort := Sort ListTermOrder.
+
+Definition flatten_eq l := ListTermSort.sort (map TermSort.sort l).
+
+Lemma perm_ldenote : forall env l l', Permutation.Permutation l l' -> ldenote env l = ldenote env l'.
+Proof.
+  intros env l l' H.
+  induction H => // ; simpl.
+  by rewrite IHPermutation.
+  ring.
+  by rewrite IHPermutation1 IHPermutation2.
+Qed.
+
+Lemma sort_ldenote : forall env l, ldenote env l = ldenote env (ListTermSort.sort l).
+Proof.
+  intros.
+  apply perm_ldenote.
+  apply Permuted_sort.
+Qed.
+
+Theorem flatten_eq_denote : forall env l, ldenote env l = ldenote env (flatten_eq l).
+Proof.
+  induction l => //.
+  unfold flatten_eq in *.
+  rewrite -sort_ldenote.
+  simpl.
+  f_equal.
+  apply sort_ldenote_M.
+  by rewrite -sort_ldenote in IHl.
+Qed.
+
+Local Definition ta := Var 1%positive.
+Local Definition tb := Var 2%positive.
+Local Definition tc := Var 3%positive.
+Local Definition td := Var 4%positive.
+Local Definition te := Var 5%positive.
+Local Definition tf := Var 6%positive.
+Local Definition tg := Var 7%positive.
+
+Local Definition expr1 := A (M ta tb) (A (R tc) (R tb)).
+Local Definition expr2 := A (A (R tc) (R tb)) (M ta tb).
+(* Eval compute in flatten_expr expr1. *)
+(* Eval compute in flatten_eq (flatten_expr expr1). *)
+(* Eval compute in (flatten_expr expr2). *)
+(* Eval compute in flatten_eq (flatten_expr expr2). *)
+
+
+
+
+(*****************************************************************************************
+ *   DECIDE EQUALITY
+ *)
+
+Fixpoint decide_list_term_eq (l l':list term): bool := match l, l' with
+  | nil , nil => true
+  | a:: qa , b :: qb => andb (term_eqb a b) (decide_list_term_eq qa qb)
+  | _, _ => false
+  end.
+
+Lemma decide_list_term_eq_impl:
+  forall env l l', 
+  decide_list_term_eq l l' = true ->
+  ldenote_M env l = ldenote_M env l'.
+Proof.
+induction l ; destruct l' ; auto => H.
+simpl in H ; discriminate.
+simpl in H ; discriminate.
+simpl in *.
+move: H; rewrite !Bool.andb_true_iff ; move=> [Ht Hl].
+apply IHl in Hl.
+move: Ht ; rewrite term_eqb_refl => -> ; rewrite Hl ; reflexivity.
+Qed.
+
+Fixpoint decide_list_list_term (l l':list (list term)) : bool := match l, l' with
+  | nil, nil => true
+  | a:: qa , b :: qb => andb (decide_list_term_eq a b) (decide_list_list_term qa qb)
+  | _, _ => false
+  end.
+
+Lemma decide_list_list_term_eq_impl : forall env l l', decide_list_list_term l l' = true -> ldenote env l = ldenote env l'.
+Proof.
+induction l ; destruct l' ; auto => H.
+simpl in H ; discriminate.
+simpl in H ; discriminate.
+simpl in *.
+move: H; rewrite !Bool.andb_true_iff ; move=> [Ht Hl].
+apply IHl in Hl.
+apply (decide_list_term_eq_impl env) in Ht.
+rewrite Ht Hl ; reflexivity.
+Qed.
+
+Definition decide_llt (l l':list (list term)) : bool := decide_list_list_term (flatten_eq l) (flatten_eq l').
+
+Definition decide_expr (e e': expr) : bool := decide_llt (flatten_expr e) (flatten_expr e').
+
+Lemma decidable_expr:
+  forall env a b,
+    decide_expr a b = true ->
+    expr_denote env a = expr_denote env b.
+Proof.
+  intros env a b Hdec.
+  unfold decide_expr in Hdec.
+  unfold decide_llt in Hdec.
+  assert(H: exists l, l = flatten_expr a).
+    eexists. reflexivity.
+  destruct H as [l Hl].
+  assert(Hld: ldenote env l = expr_denote env a).
+    rewrite flatten_expr_correct; subst => //.
+  assert(H: exists l, l = flatten_expr b).
+    eexists. reflexivity.
+  destruct H as [l' Hl'].
+  assert(Hl'd: ldenote env l' = expr_denote env b).
+    rewrite flatten_expr_correct; subst => //.
+  rewrite -Hld -Hl'd.
+  rewrite flatten_eq_denote ; symmetry ; rewrite flatten_eq_denote ; symmetry ; subst.
+  by apply decide_list_list_term_eq_impl.
+Qed.
+
+Local Example test1 : decide_llt (flatten_expr expr1) (flatten_expr expr2) = true.
+Proof.
+by compute.
+Qed.
+
+Fixpoint decide_list (l l' : list expr) : bool := match l, l' with
+  | nil, nil => true
+  | a :: qa , b :: qb => andb (decide_expr a b) (decide_list qa qb)
+  | _, _ => false
+  end.
+
+Lemma decidable_list_expr:
+  forall env a b,
+    decide_list a b = true ->
+    list_expr_denote env a = list_expr_denote env b.
+Proof.
+  induction a as [|a qa IHa] => b H.
+  destruct b.
+  reflexivity.
+  simpl in H ; congruence.
+  destruct b.
+  simpl in H ; congruence.
+  simpl in *.
+  apply Bool.andb_true_iff in H.
+  destruct H.
+  f_equal.
+  by apply decidable_expr.
+  by apply IHa.
+Qed.
+
+Definition decide_formula (f : formula) : bool := match f with
+  | Eq x y => decide_expr x y
+  | LEq x y => decide_list x y
+  end.
+
+Lemma decide_formula_impl : forall env f, decide_formula f = true -> formula_denote env f.
+Proof. move=> env [? ?| ? ?]. by apply decidable_expr. by apply decidable_list_expr. Qed.
+
+
+(********************************************************************************)
+
+Local Example test2: decide_formula (Eq expr1 expr2) = true.
+Proof.
+by compute.
+Qed.
+
+Local Example test3: decide_formula (LEq (expr1::nil) (expr2::nil)) = true.
+Proof.
+by compute.
+Qed.
+
+Close Scope Z.
