Libs/List_Ltac.v
@@ -1,0 +1,191 @@
+Set Warnings "-notation-overridden".
+Require Import Tweetnacl.Libs.List_Decidable.
+(**************************************************************************
+ * Data type for representing partial results, taken from Chlipala's CPDT
+ *)
+
+Inductive partial (P : Prop) : Set :=
+| Proved : P -> partial P
+| Uncertain : partial P.
+
+Notation "[ P ]" := (partial P) : type_scope.
+
+Notation "'Yes'" := (Proved _ _) : partial_scope.
+Notation "'No'" := (Uncertain _) : partial_scope.
+
+Local Open Scope partial_scope.
+Delimit Scope partial_scope with partial.
+
+Notation "'Reduce' v" := (if v then Yes else No) (at level 100) : partial_scope.
+
+(* Open Scope Z. *)
+
+
+(**************************************************************************
+ * Environment management tactics
+ *)
+
+Ltac inList x xs :=
+  match xs with
+  | tt => false
+  | (x, _) => true
+  | (_, ?xs') => inList x xs'
+  end.
+
+Ltac addToList x xs :=
+  let b := inList x xs in
+  match b with
+  | true => xs
+  | false => constr:((x, xs))
+  end.
+
+Ltac lookup x xs :=
+  match xs with
+  | (x, _) => constr:(1%positive)
+  | (_, ?xs') =>
+    let n := lookup x xs' in
+    constr:(Pos.succ n)
+  end.
+
+Ltac allVar xs e :=
+  match e with
+  | Z0 => xs
+  | Zpos _ => xs
+  | Zneg _ => xs
+  | _ => addToList e xs
+  end.
+
+Ltac allVars xs e :=
+  match e with
+  | Z.mul ?X ?Y =>
+    let xs := allVars xs X in
+    allVars xs Y
+  | Z.add ?X ?Y =>
+    let xs := allVars xs X in
+    allVars xs Y
+  | nil => xs
+  | ?hp :: ?qp => 
+    let xs1 := allVars xs hp in
+    allVars xs1 qp
+  | ?P = ?Q =>
+    let xs := allVars xs P in
+    allVars xs Q
+  | ?X => allVar xs X
+  | _ => xs
+  end.
+
+(**************************************************************************
+ * Reflection tactics
+ *)
+
+Ltac reifyValue env t :=
+  match t with
+  | ?X =>
+    let v := lookup X env in
+    constr:(Var v)
+  | _ => constr:(Val t)
+(*   | Zneg _ =>
+    constr:(Val t)
+  | Zpos _ =>
+    constr:(Val t) *)
+  end.
+
+Ltac reifyExpr env t :=
+  lazymatch t with
+  | Z.mul ?X ?Y =>
+    let x := reifyValue env X in
+    let y := reifyValue env Y in
+    constr:(M x y)
+  | ?X * ?Y =>
+    let x := reifyValue env X in
+    let y := reifyValue env Y in
+    constr:(M x y)
+  | Z.add ?X ?Y =>
+    let x := reifyExpr env X in
+    let y := reifyExpr env Y in
+    constr:(A x y)
+  | ?X + ?Y =>
+    let x := reifyExpr env X in
+    let y := reifyExpr env Y in
+    constr:(A x y)
+  | ?X =>
+    let x := reifyValue env X in
+    constr:(R x)
+  end.
+
+Ltac reifyList env t :=
+  match t with
+  | nil => constr:(nil:list expr)
+  | cons ?X ?Y =>
+    let x := reifyExpr env X in
+    let y := reifyList env Y in
+    constr:(x :: y)
+  end.
+
+Ltac reifyTerm env t :=
+  lazymatch t with
+  | cons ?X ?X' = cons ?Y ?Y' => 
+      let x := reifyList env (cons X X') in
+      let y := reifyList env (cons Y Y') in
+      constr:(LEq x y)
+   | ?X = ?Y =>
+      let x := reifyExpr env X in
+      let y := reifyExpr env Y in
+      constr:(Eq x y)
+  end.
+
+Ltac gather_vars :=
+  match goal with
+  | [ |- ?X ] =>
+    let xs  := allVars tt X in
+    pose xs
+  end.
+
+Ltac functionalize xs :=
+  let rec loop n xs' :=
+    lazymatch xs' with
+    | tt => constr:(fun _ : positive => 0%Z)
+    | (?x, tt) => constr:(fun _ : positive => x)
+    | (?x, ?xs'') =>
+      let f := loop (Pos.succ n) xs'' in
+      constr:(fun m : positive => if (m =? n)%positive then x else f m)
+    end in
+  loop (1%positive) xs.
+
+Local Ltac reify_debug :=
+  match goal with
+  | [ |- ?X ] =>
+    let xs  := allVars tt X in
+    let env := functionalize xs in
+    let r1  := reifyTerm xs X in
+    pose xs;
+    pose env;
+    pose r1
+  end.
+
+Ltac reify :=
+  match goal with
+  | [ |- ?X ] =>
+    let xs  := allVars tt X in
+    let env := functionalize xs in
+    let r1  := reifyTerm xs X in
+    change (formula_denote {| vars := env |} r1)
+  end.
+
+
+(**************************************************************************
+ * User interface tactics
+ *)
+
+Ltac mini_ring := intros; reify; apply decide_formula_impl; vm_compute; auto.
+
+Open Scope Z.
+Local Example example1 : forall x y, x * y = y * x.
+Proof. intros ; reify; apply decide_formula_impl; vm_compute; auto. Qed.
+
+Local Example example2 : forall x y z, x*y :: z :: nil = y * x :: z :: nil.
+Proof. mini_ring. Qed.
+
+Local Example example3 : forall x, (2*3*4*x = 3*4*2*x)%Z.
+Proof. mini_ring. Qed.
+
